	\begin{enumerate}
		\item 
			\begin{align}
				\pr{E} &= \frac{13}{52} = \frac{1}{4} 
				\\
				\pr{F} &= \frac{4}{52} = \frac{1}{13}\\
				\pr{EF} &= \frac{1}{52}\\
\because \pr{EF} &= \pr{E}\pr{F},
			\end{align}
the events are independent.
		\item
			\begin{align}
				\pr{E} &= \frac{26}{52} = \frac{1}{2}
				\\
				\pr{F} &= \frac{4}{52} = \frac{1}{13} \\
				\pr{EF} &= \frac{2}{52} = \frac{1}{26} \\
\because \pr{EF} &= \pr{E}\pr{F},
			\end{align}
			$E$ and $F$ are independent.  
		\item
			\begin{align}
				\pr{E} &= \frac{8}{52} = \frac{2}{13} \\
				\pr{F} &= \frac{8}{52} = \frac{2}{13}\\
				\pr{EF} &= \frac{4}{52} = \frac{1}{13}\\
				\pr{E}\pr{F} &= \frac{2}{13} \times \frac{2}{13} = \frac{4}{169}\\
				\therefore~\pr{EF} &\neq \pr{E}\pr{F}
			\end{align}	
			and   $E$ and $F$ are not independent.  
	\end{enumerate}
