\begin{align}
E(X)&=\sum_{k=0}^{5} kp_X(k)\\
&=0\left(\frac{1}{6}\right)+1\left(\frac{5}{18}\right)+2\left(\frac{2}{9}\right)+3\left(\frac{1}{6}\right)+4\left(\frac{1}{9}\right)+5\left(\frac{1}{18}\right)\\
&=\frac{35}{18}
\label{eq:12.13.3.37,4}
\end{align}
\begin{align}
E(X^2)&=\sum_{k=0}^{5} k^2p_X(k)\\
&=0^2\left(\frac{1}{6}\right)+1^2\left(\frac{5}{18}\right)+2^2\left(\frac{2}{9}\right)+3^2\left(\frac{1}{6}\right)+4^2\left(\frac{1}{9}\right)+5^2\left(\frac{1}{18}\right)\\
&=\frac{105}{18}
\label{eq:12.13.3.37,7}
\end{align}
From \eqref{eq:12.13.3.37,4} and \eqref{eq:12.13.3.37,7}.
\begin{align}
\sigma^2&=E(X^2)-[E(X)]^2\\
&=\frac{105}{18}-\left(\frac{35}{18}\right)^2\\
&=\frac{665}{324}
\end{align}
