\begin{enumerate}
\item
\begin{equation}
\pr{A|B}= \frac{\pr{AB}}{\pr{B}}= \frac{3}{4}
\end{equation}
\item
\begin{equation}
\pr{B|A}= \frac{\pr{AB}}{\pr{A}}= \frac{1}{2}
\end{equation}
\item From 
\eqref{eq:axiom-cond-prime},
\begin{align}
\pr{A^{\prime}|B}= \frac{\pr{B}-\pr{AB}}{\pr{B}}
= \frac{1}{4}
\end{align}
\item
\begin{align}
\pr{A^{\prime}|B^{\prime}}&= \frac{\pr{A^{\prime} B^{\prime}}}{\pr{B^{\prime}}}\\
&=\frac{\pr{A + B}^{\prime}}{\pr{B^{\prime}}}
=\frac{1- \pr{A + B}}{1-\pr{B}}
\\
&= \frac{5}{8} 
\end{align}
using 
\eqref{eq:axiom_sum_AB} in the numerator.
\end{enumerate}

