From the given information, 
\begin{align}
p_X(0)=p_X(1)=p, 
p_X(2) = 1 - 2p.
\end{align}
Then,
\begin{align}
E\brak{X} &= \sum_{k=0}^2 kp_X(k)\\
&= 0p_X(0) + 1p_X(1) +2p_X(2)\\
&= 2-3p \label{eq:exemplar/12/13/3/36/1}
\end{align}
and
\begin{align}
E\brak{X^2} &= \sum_{k=0}^2 k^2p_X(k)\\
&= 0p_X(0) + 1p_X(1) +4p_X(2)\\
&= 4-7p \label{eq:exemplar/12/13/3/36/2}
\end{align}
Since
\begin{align}
E\brak{X} = E\brak{X^2},
\end{align}
from \eqref{eq:exemplar/12/13/3/36/1} and \eqref{eq:exemplar/12/13/3/36/2}
\begin{align}
2-3p &= 4-7p\\
\implies p &= \frac{1}{2}
\end{align}


