\section{Definitions}
\begin{enumerate}[label=\thesection.\arabic*,ref=\thesection.\theenumi]
\numberwithin{equation}{enumi}
\numberwithin{figure}{enumi}
\numberwithin{table}{enumi}

\item 
\begin{align}
	0 \le \pr{A} \le 1	
\end{align}
\item If $AB = 0$,
\begin{align}
	\pr{A+B} = \pr{A} + \pr{B}.
\end{align}
\item If $A, B$ are independent,
\begin{align}
	\pr{AB} = \pr{A}\pr{B}
\end{align}
\item 
\begin{align}
	\pr{A | B} = \frac{\pr{AB}}{\pr{B}}
\end{align}
\end{enumerate}
\section{Boolean Logic}
\begin{enumerate}[label=\thesection.\arabic*,ref=\thesection.\theenumi]
\numberwithin{equation}{enumi}
\numberwithin{figure}{enumi}
\numberwithin{table}{enumi}
\item 
\begin{align}
	A + A^{\prime} = 1
\end{align}
\item 
\begin{align}
A^{\prime}B^{\prime} &=  \brak{A+B}^{\prime}
\end{align}
\item 
\begin{align}
A+B &= A\brak{B+B^{\prime}} + B
\\
&= B \brak{A +1} + A B^{\prime}
\\
&=B + A B^{\prime}
\end{align}
\item 
\begin{align}
A = A \brak{B+B^{\prime}} =  AB + AB^{\prime}
\label{eq:axiom_sum_A}
\end{align}
and 
\begin{align}
\brak{ AB}\brak{  AB^{\prime}} = 0, \because BB^{\prime} = 0
\label{eq:axiom_sum_AB0}
\end{align}
Hence, $AB$ and $AB^{\prime}$ are mutually exclusive. 
\newpage 
\item 
Let A, B and C be three events.

Let X be the event that exactly one of A, B and C occurs.

Let Y be the event that at least one of A, B or C occur.

Let Z be the event that at least two of A, B or C occur.
\begin{align}
	Y &=A+B+C
\end{align}
Similarly,
\begin{align}
	Z &=AB+BC+CA
\end{align}
And,
\begin{align}
    X&=(AB^\prime C^\prime+A^\prime BC^\prime+A^\prime B^\prime C)
	\label{eq:axiom_occurrence_of_exactly_one}
\end{align}
\end{enumerate}
\newpage
\section{Properties}
\begin{enumerate}[label=\thesection.\arabic*,ref=\thesection.\theenumi]
\numberwithin{equation}{enumi}
\numberwithin{figure}{enumi}
\numberwithin{table}{enumi}
\item 
\begin{align}
	\pr{A^{\prime}} = 1 - \pr{A}.
\end{align}
\item
\begin{align}
\pr{A^{\prime}B^{\prime}} &=  \pr{\brak{A+B}^{\prime}} 
\\
&= 1 - \pr{A+B} 
\label{eq:axiom_sum_one}
\end{align}
\item 
\begin{align}
\pr{A+B} &= \pr{B + A B^{\prime} }
\\
&=\pr{B}+\pr{ A B^{\prime} } 
\label{eq:axiom_sum_two}
\\
&\because B \brak{ A B^{\prime} } = 0
\end{align}
\item
\begin{align}
\pr{A} = \pr{AB} + \pr{AB^{\prime}}
\\
\implies 
\pr{AB^{\prime}} =  \pr{A} - \pr{AB}
\label{eq:axiom_sum_ABp}
\end{align}
\item Substituting \eqref{eq:axiom_sum_ABp} in \eqref{eq:axiom_sum_two}, 
	\begin{align}
\pr{A+B} &= \pr{A} + \pr{B} - \pr{AB} 
\label{eq:axiom_sum_AB}
\end{align}
\end{enumerate}
