\begin{enumerate}[label=\thesubsection.\arabic*,ref=\thesubsection.\theenumi]
\item 
\begin{align}
	\pr{A | B} = \frac{\pr{AB}}{\pr{B}}
\label{eq:axiom-cond}
\end{align}
If $A$ and $B$ are independent, from 
\eqref{eq:axiom-cond}
and 
\eqref{eq:axiom-ind},
\begin{align}
	\pr{A | B} = \frac{\pr{A}\pr{B}}{\pr{B}}={\pr{A}}
\label{eq:axiom-cond-ind}
\end{align}
\item 
\begin{align}
	\pr{A' | B} = \frac{\pr{A'B}}{\pr{B}} = \frac{\pr{B}-\pr{AB}}{\pr{B}}
\label{eq:axiom-cond-prime}
\end{align}
\item Total probability
	\begin{align}
		\pr{A} = \sum_{i=1}^{2}\pr{E_i}\pr{A|E_i}
\label{eq:axiom-tot-prob}
\end{align}
\item Bayes' Theorem
\begin{align}
	\pr{E_1|A} &= \frac{\pr{E_1}\pr{A|E_1}}{\sum_{i=1}^{2}\pr{E_i}\pr{A|E_i}}
\label{eq:axiom-bayes}
\end{align}
\item Let $X, Y \in \cbrak{0,1}$ be two random variables.  Then, 
\begin{align}
	\label{eq:12/13/3/43/yixj-def}
	  \pr{Y=1|X=0}\triangleq  p_{Y|X}\brak{1|0}
\end{align}
\item 
\begin{align}
	   p_{Y|X}\brak{1|0}
	   &=
	   \frac{p_{X,Y}\brak{0,1}}{p_{X}\brak{0}}
	   =
	   \frac{p_{X}\brak{0}-p_{X,Y}\brak{0,0}}{p_{X}\brak{0}}
	   \\
	   &=
	   1-\frac{p_{X,Y}\brak{0,0}}{p_{X}\brak{0}} = 1-p_{Y|X}\brak{0|0}
	\label{eq:12/13/3/43/yixj}
\end{align}
\end{enumerate}
