There are two conditions, 
\begin{enumerate}
\item  $s$ is chosen first:
\begin{align}
\pr{r\le p\,|\,s\le p} = \frac{\pr{r \le p, \, s \le p}}{\pr{s \le p}}
\end{align}
\begin{enumerate}
\item $p<1$:
This case is never possible as $s,r \ge 1$
\item $1 \le p \le n$:
Then we can say that,
\begin{align}
\pr{r \le p, \, s \le p} &= \frac{p(p-1)}{n(n-1)} \label{eq:12/13/3/34/1},\\
\pr{s \le p} &= \frac{p}{n} \label{eq:12/13/3/34/2}
\end{align}
From \eqref{eq:12/13/3/34/1} and \eqref{eq:12/13/3/34/2}:
\begin{align}
\pr{r\le p|s\le p} &= \frac{\pr{r \le p, \, s \le p}}{\pr{s \le p}}\\
&= \frac{\frac{p(p-1)}{n(n-1)}}{\frac{p}{n}}
=\frac{p-1}{n-1}
\end{align}
\item $p>n$:
\begin{align}
\pr{r \le p, \, s \le p} &= 1 \label{eq:12/13/3/34/3},\\
\pr{s \le p} &= 1 \label{eq:12/13/3/34/4}
\end{align}
From \eqref{eq:12/13/3/34/3} and \eqref{eq:12/13/3/34/4}:
\begin{align}
\pr{r\le p|s\le p} &= \frac{\pr{r \le p, \, s \le p}}{\pr{s \le p}}\\
&= 1 
\end{align}
\end{enumerate}
\item  r is chosen first:
\begin{align}
\pr{r\le p|s\le p} = \frac{\pr{r \le p, \, s \le p}}{\pr{s \le p}}
\end{align}
\begin{enumerate}
\item $p<1$:
This case is never possible as $r,s \ge 1$
\item $1 \le p \le n$:
\begin{align}
\pr{r \le p, \, s \le p} &= \frac{p(p-1)}{n(n-1)} \label{eq:12/13/3/34/5},\\
\pr{s \le p} &= \frac{p-1}{n-1} \label{eq:12/13/3/34/6}
\end{align}
From \eqref{eq:12/13/3/34/5} and \eqref{eq:12/13/3/34/6}:
\begin{align}
\pr{r\le p|s\le p} &= \frac{\pr{r \le p, \, s \le p}}{\pr{s \le p}}\\
&= \frac{\frac{p(p-1)}{n(n-1)}}{\frac{p}{n}}
=\frac{p}{n}
\end{align}
\item $p>n$:
\begin{align}
\pr{r \le p, \, s \le p} &= 1 \label{eq:12/13/3/34/7},\\
\pr{s \le p} &= 1 \label{eq:12/13/3/34/8}
\end{align}
From \eqref{eq:12/13/3/34/7} and \eqref{eq:12/13/3/34/8}:
\begin{align}
\pr{r\le p|s\le p} &= \frac{\pr{r \le p, \, s \le p}}{\pr{s \le p}}\\
&= 1 
\end{align}
\end{enumerate}
\end{enumerate}





















