From the axiom of total probability,
\begin{align}
    &\sum_{i = 1}^{6} p_X(i) = 1\\
    \implies &\sum_{i = 1}^{3} ki^2 + \sum_{i = 4}^{6} 2ki = 1\\
    \implies &k + 4k + 9k + 8k + 10k + 12k = 1\\
    \implies &k = \frac{1}{44}
\end{align}
Therefore,
\begin{align*}
    p_X(x) =
    \begin{cases}
        \frac{x^2}{44} &\text{for } x = 1,2,3\\
        \frac{2x}{44} &\text{for } x = 4,5,6\\
        0 & \text{otherwise}
    \end{cases}
\end{align*}
\begin{enumerate}
    \item 
    \begin{align}
        E\brak{X} 
        &= \sum_{i = 1}^{6} ip_X(i)\\
        &= \frac{95}{22}\\
    \end{align}
    \item 
    \begin{align}
        E\brak{3X^2} &= 3E\brak{X^2}\\
        &= 3\sum_{i = 1}^{6} i^2 p_{X}(i)\\
        &= \frac{2724}{44}\\
    \end{align}
    \item The CDF
    \begin{align}
        F_X(x) &= \sum_{i = 1}^{x} p_X(i)\\ &= 
        \begin{cases}
            \sum_{i = 1}^{x} \frac{i^2}{44} & \text{if } x \leq 3\\
            \sum_{i = 1}^{3} \frac{i^2}{44} + \sum_{i = 4}^{x} \frac{2i}{44} & \text{if } x \geq 4
        \end{cases}\\
        &=
        \begin{cases}
            \frac{x(x+1)(2x+1)}{6 \times 44} & \text{if } x \leq 3\\
            \frac{14}{44} + \frac{x(x+1)}{44} - \frac{3 \times 4}{44} & \text{if } x \geq 4
        \end{cases}\\
        &=
        \begin{cases}
            \frac{x(x+1)(2x+1)}{264} & \text{if } x \leq 3\\
            \frac{x(x+1) + 2}{44} & \text{if } x \geq 4
        \end{cases}
    \end{align}
   Therefore, 
    \begin{align}
        \pr{X \geq 4} &= 1 - \pr{X \leq 3}\\
        &= 1 - F_X\brak{3}\\
        &= 1 - \frac{3 \times 4 \times 7}{264}\\
        &= \frac{15}{22}
    \end{align}
\end{enumerate}

