\begin{align}
	\because
\pr{A} = \frac{1}{2},\ \pr{B} = \frac{1}{3},
\\
          \pr{AB} = \pr{A}\pr{B}=\frac{1}{6}
\end{align}
     $\because A,B$ are independent.
 \begin{enumerate}
 \item     From  
\eqref{eq:axiom_sum_AB},
     \begin{align}
 \pr{A+B}          
          = \frac{1}{2} + \frac{1}{3} -\frac{1}{6} = \frac{2}{3}
          \end{align}
               \item 
               \begin{align}
		       \pr{AB^{\prime}+A^{\prime}B}&=
                     \pr{AB^{\prime}}+\pr{A^{\prime}B}
		     \\
                    &= \pr{A}\pr{B^{\prime}}+\pr{A^{\prime}}\pr{B}
		    \\
                    &= \pr{A}+\pr{B}-2\pr{A}\pr{B} = 
                     \frac{1}{2}
               \end{align}
 \end{enumerate}

      

