\begin{enumerate}
\item \begin{align}
p_1p_2&=\pr{E_1}\pr{E_2}\\
&=\pr{E_1E_2}
\end{align}
So, $E_1$ and $E_2$ occur simultaneously.
\item \begin{align}
(1 - p_1)(p_2) &= \pr{E_1^\prime}\pr{E_2} \\
&= \pr{{E_1^\prime}E_2}
\end{align}
So $E_1$ does not occur but $E_2$  occurs.
\item \begin{align}
1 - (1 - p_1)(1 - p_2) &= 1 - \pr{E_1^\prime} \pr{E_2^\prime} \\
&= 1 - \pr{E_1^\prime \ E_2^\prime} \\
&= \pr{E_1+E_2} 
\end{align}
So, either $E_1$ or $E_2$ or both $E_1$ and $E_2$  occurs.
\item \begin{align}
p_1 + p_2 - 2p_1p_2 &= \pr{E_1} + \pr{E_2} - 2\pr{E_1} \pr{E_2} \\
&=  \pr{E_1}-\pr{E_1}\pr{E_2}+ \pr{E_2} - \pr{E_1} \pr{E_2}\\
&= \pr{E_1}\brak{1-\pr{E_2}}+\pr{E_2} \brak{1-\pr{E_1}}\\
&=\pr{E_1}\pr{E_2^\prime}+\pr{E_2}\pr{E_1^\prime}\\
&=\pr{E_1E_2^\prime+E_1^\prime E_2}
\end{align}
So, either $E_1$ or $E_2$ occurs but not both.
\end{enumerate}



