From \eqref{eq:axiom-cond},
\begin{align}
\pr{AB} = \frac{3}{5}\times \frac{1}{2} = \frac{3}{10}
\end{align}
From \eqref{eq:axiom_sum_A},
\begin{align}
	\pr{A'B} =  
 \frac{3}{5}- \frac{3}{10}
 =\frac{3}{10}
\end{align}
From \eqref{eq:axiom_sum_AB},
\begin{align}
\pr{A} = \frac{4}{5}+ \frac{3}{10}
- \frac{3}{5} = 
 \frac{1}{2}.  
\end{align}
Again, using \eqref{eq:axiom_sum_A},
\begin{align}
	\pr{AB'} =  \frac{1}{2} - \frac{3}{10} = \frac{1}{5}.
\end{align}
Thus, 
	using \eqref{eq:demorgan},
\begin{align}
\pr{A + B}^{\prime} + \pr{A^{\prime} + B} 
	&=1 -\frac{1}{5} + 1- \frac{3}{10}
= \frac{3}{2}.
\end{align}
