		\begin{table}[htb]
		\centering
		\input{ncert/12/13/1/11/tables/Table1.tex}
		\caption{}
		\label{tab:ncert/12/13/1/11/table1}
		\end{table}
	See 	
		\tabref{tab:ncert/12/13/1/11/table1}.
		\begin{enumerate}
		\item
		\begin{align}
			\pr{\cond{E}{F}} = \frac{\pr{EF}}{\pr{F}}
		 = \frac{1/6}{1/3}
		 = 1/2
		\end{align}
		\item
		\begin{align}
		\pr{F|E} = \frac{\pr{EF}}{\pr{E}}
         = \frac{1/6}{1/2}
         = 1/3
        \end{align}
		\item
		\begin{align}
			\pr{E|G} = \frac{\pr{EG}}{\pr{G}}
        = \frac{1/3}{2/3}
        = 1/2
        \end{align}
        \item
        \begin{align}
		\pr{G|E} = \frac{\pr{EG}}{\pr{E}}
        = \frac{1/3}{1/2}
        = 2/3
        \end{align}
        \item
        \begin{align}
		\because	\pr{(E+F)G} &= \pr{EG+FG}= \pr{EG}+\pr{FG}-\pr{EFG},
	\nonumber	\\
		 &= \frac{1}{3} + \frac{1}{3} - \frac{1}{6}
		 = \frac{1}{2}
		 \\
		\pr{(E+F)|G} &= \frac{\pr{(E+F)G}}{\pr{G}}
		 = \frac{1/2}{2/3}
		 = \frac{3}{4}
		\end{align}
		\item
		\begin{align}
			\pr{EF|G} &= \frac{\pr{EFG}}{\pr{G}}
         = \frac{1/6}{2/3}
			= \frac{1}{4}
		\end{align}

\end{enumerate}
